proved load/save conjunction lemma

split/model_lemmas.v
@@ -477,181 +477,133 @@ Notation "'ALL' x .. y , P " :=
 
 
 Inductive cut_resource_rmap_exp (sh:share) l (len:Z) (bl: list memval): rmap -> rmap -> Prop :=
-| cut_resource_exp_intro: forall r_mapsto r1 r2 (Hl: Z.of_nat (Datatypes.length bl) = len),
+| cut_resource_exp_intro: forall r_mapsto 
+  r1 r2 (Hl: Z.of_nat (Datatypes.length bl) = len),
   (((ALL y, jam (adr_range_dec l len)
       (fun l' => yesat NoneP (VAL (nth (Z.to_nat (snd l' - snd l)) bl Undef)) sh l') noat y) && noghost) r_mapsto)%pred ->
   join r_mapsto r1 r2 ->
   cut_resource_rmap_exp sh l len bl r1 r2.
 
-Inductive cut_nonlock_rmap_exp (sh:share) l (len:Z) (bl: list memval): rmap -> rmap -> Prop :=
-| cut_nonlock_exp_intro: forall r_mapsto r1 r2 (Hl: Z.of_nat (Datatypes.length bl) = len),
-(((ALL y, jam (adr_range_dec l len) (fun i : address => shareat i sh && nonlockat i) noat y) && noghost) r_mapsto)%pred ->
-join r_mapsto r1 r2 ->
-cut_nonlock_rmap_exp sh l len bl r1 r2.
-
-
-
-
-(* Inductive cut_resource_rmap (sh:share) l (len:Z): rmap -> rmap -> Prop :=
-| cut_resource_intro: forall (bl: list memval) r_mapsto r1 r2 (Hl: Z.of_nat (Datatypes.length bl) = len),
-  ((ALL y, jam (adr_range_dec l len)
-      (fun l' => yesat NoneP (VAL (nth (Z.to_nat (snd l' - snd l)) bl Undef)) sh l') noat y) && noghost) r_mapsto ->
-  join r_mapsto r1 r2 ->
-  cut_resource_rmap sh l len r1 r2. *)
-
 Inductive cut_resource_rmap (sh:share) l (len:Z): rmap -> rmap -> Prop :=
-| cut_resource_intro: forall (bl: list memval) r1 r2,
-cut_resource_rmap_exp sh l len bl r1 r2 ->
-  cut_resource_rmap sh l len r1 r2.
-
-Inductive cut_nonlock_rmap (sh:share) l (len:Z): rmap -> rmap -> Prop :=
-| cut_nonlock_intro: forall (bl: list memval) r1 r2,
-cut_nonlock_rmap_exp sh l len bl r1 r2 ->
-cut_nonlock_rmap sh l len r1 r2.
+  | cut_resource_intro: forall (bl: list memval) r1 r2,
+    cut_resource_rmap_exp sh l len bl r1 r2 ->
+    cut_resource_rmap sh l len r1 r2.
   
-
-(* Inductive cut_resource_rmap (sh:share) ls: rmap -> rmap -> Prop :=
-| cut_resource_intro: forall (b: memval) r_mapsto r1 r2,
-  ((ALL y, jam (fun l' => in_dec EqDec_address l' ls)
-      (fun l' => yesat NoneP (VAL b) sh l') noat y) && noghost) r_mapsto ->
-  join r_mapsto r1 r2 ->
-  cut_resource_rmap sh ls r1 r2. *)
-(* TODO: b in fact can be any *)
+Inductive cut_resource_rejoin (sh:share) l m v: rmap -> rmap -> Prop :=
+| cut_resource_rejoin_exp_intro:
+    forall r_rem r_rem' r_mapsto' r1 r2,
+    address_mapsto m v sh l r_mapsto' ->
+    cut_resource_rmap sh l (size_chunk m) r_rem r1 ->
+    necR r_rem r_rem' ->
+    join r_rem' r_mapsto' r2->
+    cut_resource_rejoin sh l m v r1 r2.
 
 Lemma cut_resource_rmap_unique: forall sh l len r1 r2 r,
 cut_resource_rmap sh l len r1 r ->
 cut_resource_rmap sh l len r2 r ->
 r1 = r2.
 Proof.
-intros. inv H. rename H1 into H.
-inv H0. rename H1 into H0. inv H. inv H0.
-pose proof join_join_sub H2.
-pose proof join_join_sub H3.
-assert (r_mapsto = r_mapsto0).
-{ apply rmap_ext.
-  + apply join_level in H2. apply join_level in H3.
-    destruct H2, H3. congruence.
-  + intros. hnf in H1. destruct H1, H.
+  intros. inv H. rename H1 into H.
+  inv H0. rename H1 into H0. inv H. inv H0.
+  pose proof join_join_sub H2.
+  pose proof join_join_sub H3.
+  assert (r_mapsto = r_mapsto0).
+  { apply rmap_ext.
+    + apply join_level in H2. apply join_level in H3.
+      destruct H2, H3. congruence.
+    + intros. hnf in H1. destruct H1, H.
+      apply resource_at_join with (loc:=l0) in H2.
+      apply resource_at_join with (loc:=l0) in H3.
+      specialize (H1 l0).
+      specialize (H l0). hnf in H1, H.
+      if_tac in H1;subst.
+      * destruct H1, H. rewrite H1, H. f_equal. apply proof_irr.
+        f_equal. rewrite H1, H in *. inv H2; inv H3; try congruence.
+      * do 3 red in H,H1.
+        apply resource_at_join_sub with (l:=l0) in H0. 
+        eapply join_sub_same_identity; eauto.
+        - apply identity_unit'; auto.
+        - apply (resource_at_join_sub _ _ l0) in H4.
+          eapply join_sub_unit_for; eauto.
+          apply identity_unit'; auto.
+    + destruct H1, H. 
+      eapply same_identity; auto.
+      * destruct H0 as [? H0%ghost_of_join].
+        rewrite (H5 _ _ H0) in H0. eauto.
+      * destruct H4 as [? H4%ghost_of_join].
+        rewrite (H6 _ _ H4) in H4; eauto.
+  }
+  subst r_mapsto0. clear H0 H4 H.
+  apply rmap_ext.
+  { apply join_level in H2. apply join_level in H3.
+    destruct H2, H3. congruence. }
+  { intros. hnf in H1. destruct H1.
+    specialize (H l0).
     apply resource_at_join with (loc:=l0) in H2.
-    apply resource_at_join with (loc:=l0) in H3.
-    specialize (H1 l0).
-    specialize (H l0). hnf in H1, H.
-    if_tac in H1;subst.
-    * destruct H1, H. rewrite H1, H. f_equal. apply proof_irr.
-      f_equal. rewrite H1, H in *. inv H2; inv H3; try congruence.
-    * do 3 red in H,H1.
-      apply resource_at_join_sub with (l:=l0) in H0. 
-      eapply join_sub_same_identity; eauto.
-      - apply identity_unit'; auto.
-      - apply (resource_at_join_sub _ _ l0) in H4.
-        eapply join_sub_unit_for; eauto.
-        apply identity_unit'; auto.
-  + destruct H1, H. 
-    eapply same_identity; auto.
-    * destruct H0 as [? H0%ghost_of_join].
-      rewrite (H5 _ _ H0) in H0. eauto.
-    * destruct H4 as [? H4%ghost_of_join].
-      rewrite (H6 _ _ H4) in H4; eauto.
-}
-subst r_mapsto0. clear H0 H4 H.
-apply rmap_ext.
-{ apply join_level in H2. apply join_level in H3.
-  destruct H2, H3. congruence. }
-{ intros. hnf in H1. destruct H1.
-  specialize (H l0).
-  apply resource_at_join with (loc:=l0) in H2.
-  apply resource_at_join with (loc:=l0) in H3. hnf in H.
-  if_tac in H.
-  + hnf in H. destruct H as [rsh H]. rewrite H in *.
-    inv H2; inv H3; try congruence;rewrite <- H10 in H9; inv H9.
-    - apply join_comm in RJ. apply join_comm in RJ0.
-      pose proof join_canc RJ RJ0.
-      subst sh0. f_equal. apply proof_irr.
-    - apply join_comm in RJ. apply join_comm in RJ0.
-      pose proof join_canc RJ RJ0.
-      subst sh0. contradiction.
-    - apply join_comm in RJ. apply join_comm in RJ0.
-      pose proof join_canc RJ RJ0.
-      subst sh0. contradiction.
-    - apply join_comm in RJ. apply join_comm in RJ0.
-      pose proof join_canc RJ RJ0.
-      subst sh0. f_equal. apply proof_irr.
-  + apply H in H2. apply H in H3. congruence.
-}
-{ hnf in H1. destruct H1.
-  apply ghost_of_join in H2.
-  apply ghost_of_join in H3.
-  apply H0 in H2. apply H0 in H3.
-  congruence. }
+    apply resource_at_join with (loc:=l0) in H3. hnf in H.
+    if_tac in H.
+    + hnf in H. destruct H as [rsh H]. rewrite H in *.
+      inv H2; inv H3; try congruence;rewrite <- H10 in H9; inv H9.
+      - apply join_comm in RJ. apply join_comm in RJ0.
+        pose proof join_canc RJ RJ0.
+        subst sh0. f_equal. apply proof_irr.
+      - apply join_comm in RJ. apply join_comm in RJ0.
+        pose proof join_canc RJ RJ0.
+        subst sh0. contradiction.
+      - apply join_comm in RJ. apply join_comm in RJ0.
+        pose proof join_canc RJ RJ0.
+        subst sh0. contradiction.
+      - apply join_comm in RJ. apply join_comm in RJ0.
+        pose proof join_canc RJ RJ0.
+        subst sh0. f_equal. apply proof_irr.
+    + apply H in H2. apply H in H3. congruence.
+  }
+  { hnf in H1. destruct H1.
+    apply ghost_of_join in H2.
+    apply ghost_of_join in H3.
+    apply H0 in H2. apply H0 in H3.
+    congruence. }
 Qed.
 
 
-(* Lemma cut_resource_rmap_unique_rev: forall sh l len r1 r2 r,
-cut_resource_rmap sh l len r r1 ->
-cut_resource_rmap sh l len r r2 ->
-r1 = r2.
+Lemma cut_resource_sem: forall r m v1 v2 sh l P,
+  (address_mapsto m v1 sh l * (address_mapsto m v2 sh l -* P))%pred r ->
+  forall r', cut_resource_rejoin sh l m v2 r r' -> P r'.
 Proof.
-intros. inv H. rename H1 into H.
-inv H0. rename H1 into H0. inv H. inv H0.
-pose proof join_join_sub H2.
-pose proof join_join_sub H3.
-assert (r_mapsto = r_mapsto0).
-{ apply rmap_ext.
-  + apply join_level in H2. apply join_level in H3.
-    destruct H2, H3. congruence.
-  + intros. hnf in H1. destruct H1, H.
-    apply resource_at_join with (loc:=l0) in H2.
-    apply resource_at_join with (loc:=l0) in H3.
-    specialize (H1 l0).
-    specialize (H l0). hnf in H1, H.
-    if_tac in H1;subst.
-    * destruct H1, H. rewrite H1, H. f_equal. apply proof_irr.
-      f_equal. rewrite H1, H in *. inv H2; inv H3; try congruence.
-    * do 3 red in H,H1.
-      apply resource_at_join_sub with (l:=l0) in H0. 
-      eapply join_sub_same_identity; eauto.
-      - apply identity_unit'; auto.
-      - apply (resource_at_join_sub _ _ l0) in H4.
-        eapply join_sub_unit_for; eauto.
-        apply identity_unit'; auto.
-  + destruct H1, H. 
-    eapply same_identity; auto.
-    * destruct H0 as [? H0%ghost_of_join].
-      rewrite (H5 _ _ H0) in H0. eauto.
-    * destruct H4 as [? H4%ghost_of_join].
-      rewrite (H6 _ _ H4) in H4; eauto.
-}
-subst r_mapsto0. clear H0 H4 H.
-apply rmap_ext.
-{ apply join_level in H2. apply join_level in H3.
-  destruct H2, H3. congruence. }
-{ intros. hnf in H1. destruct H1.
-  specialize (H l0).
-  apply resource_at_join with (loc:=l0) in H2.
-  apply resource_at_join with (loc:=l0) in H3. hnf in H.
-  if_tac in H.
-  + hnf in H. destruct H as [rsh H]. rewrite H in *.
-    inv H2; inv H3; try congruence;rewrite <- H10 in H9; inv H9.
-    - apply join_comm in RJ. apply join_comm in RJ0.
-      pose proof join_canc RJ RJ0.
-      subst sh0. f_equal. apply proof_irr.
-    - apply join_comm in RJ. apply join_comm in RJ0.
-      pose proof join_canc RJ RJ0.
-      subst sh0. contradiction.
-    - apply join_comm in RJ. apply join_comm in RJ0.
-      pose proof join_canc RJ RJ0.
-      subst sh0. contradiction.
-    - apply join_comm in RJ. apply join_comm in RJ0.
-      pose proof join_canc RJ RJ0.
-      subst sh0. f_equal. apply proof_irr.
-  + apply H in H2. apply H in H3. congruence.
-}
-{ hnf in H1. destruct H1.
-  apply ghost_of_join in H2.
-  apply ghost_of_join in H3.
-  apply H0 in H2. apply H0 in H3.
-  congruence. }
-Qed. *)
+  intros.
+  destruct H as [r_maps [r_rem [H1 [H2 H3]]]]. inv H0.
+  eapply H3.
+  3:{ apply H. }
+  2:{ apply H6. }
+  assert (cut_resource_rmap sh l (size_chunk m) r_rem r).
+  { destruct H2 as [bl H2]. eapply cut_resource_intro with (bl:=bl).
+    destruct H2 as [[H2 ?] ?]. simpl in H2. destruct H2.
+    apply cut_resource_exp_intro with (r_mapsto := r_maps);auto.
+    { rewrite H2. rewrite size_chunk_conv. reflexivity. }
+    { split;auto. }
+  }
+  pose proof cut_resource_rmap_unique _ _ _ _ _ _ H4 H0.
+  subst. auto.
+Qed.
+
+
+Lemma cut_resource_sem_inv: forall r m v1 v2 sh l bl (P: pred rmap) r_rem,
+  cut_resource_rmap_exp sh l (size_chunk m) bl r_rem r ->
+  decode_val m bl = v1 -> (align_chunk m | snd l) ->
+  (forall r', cut_resource_rejoin sh l m v2 r r' -> P r') ->
+  (address_mapsto m v1 sh l * (address_mapsto m v2 sh l -* P))%pred r.
+Proof.
+  intros. inversion H as [bm]. subst.
+  inversion H. subst. exists r_mapsto, r_rem. split;auto. split.
+  - hnf. exists bl. destruct H0. split;auto. split;auto. simpl;auto.
+    rewrite size_chunk_conv in Hl.  repeat split;auto.
+    rewrite <- Nat2Z.id at 1. rewrite Hl0. reflexivity.
+  - hnf. intros r_rem' r_maps' r'. intros.
+    apply H2. eapply cut_resource_rejoin_exp_intro; try eassumption.
+    apply cut_resource_intro with (bl:=bl);auto.
+Qed.
+
+
 
 Lemma share_resource_join_aux: forall sh1 sh2 sh3 sh5 sh,
 join sh1 sh3 sh -> join sh2 sh5 sh -> join (Share.lub sh1 sh2) (Share.glb sh (Share.comp (Share.lub sh1 sh2))) sh.
@@ -694,12 +646,310 @@ Proof.
 Qed.
 
 
+Lemma cut_resource_map_preserve_necR_aux {sh lbase len bm}:
+  forall n r_rem r r_rem' r',
+  relation_power n age r_rem r_rem' ->
+  relation_power n age r r' ->
+  cut_resource_rmap_exp sh lbase len bm r_rem r ->
+  cut_resource_rmap_exp sh lbase len bm r_rem' r'.
+Proof.
+  induction n;intros.
+  - simpl in H0. simpl in H. subst. tauto.
+  - destruct H as [r_rem'' [? ?]].
+    destruct H0 as [r'' [? ?]].
+    apply (IHn _ _ _ _ H2 H3).
+    { inv H1.
+      assert (exists r_mapsto'', age r_mapsto r_mapsto'').
+      { eapply level_age_fash. apply join_level in H5.
+        apply age_level in H0. rewrite (proj1 H5). apply H0. }
+      destruct H1 as [r_mapsto'' H1].
+      eapply cut_resource_exp_intro with (r_mapsto:= r_mapsto'');auto.
+      2:{ eapply age1_join_eq;[apply H5|..];auto. }
+      hnf in H.
+      destruct H4. split.
+      + intros l. specialize (H4 l).
+        hnf in H4. hnf. if_tac.
+        { destruct H4. exists x. hnf in H4.
+          hnf. simpl. epose proof age1_YES _ _ _ _ _ _ H1.
+          apply H8 in H4. auto. }
+        { epose proof age1_resource_at_identity _ _ _ H1.
+          apply H8 in H4. auto. }
+      + epose proof age1_ghost_of_identity _ _ H1.
+        apply H7 in H6. auto.
+    }
+Qed.
+
+
+Lemma cut_resource_map_preserve_necR {sh lbase len bm}:
+  forall r_rem r r_rem' r',
+  cut_resource_rmap_exp sh lbase len bm r_rem r ->
+  necR r_rem r_rem' ->
+  necR r r' ->
+  level r' = level r_rem' ->
+  cut_resource_rmap_exp sh lbase len bm r_rem' r'.
+Proof.
+  intros. apply necR_power_age in H0. apply necR_power_age in H1.
+  destruct H0 as [m H0]. destruct H1 as [n H1].
+  assert (m = n).
+  { inv H. apply join_level in H4.
+    apply relation_power_level in H0. apply relation_power_level in H1.
+    omega. }
+  subst m. eapply cut_resource_map_preserve_necR_aux;try eassumption.
+Qed.
+
+Lemma address_mapsto_preserve_necR {sh lbase m v}:
+  forall r_mapsto' r_mapsto,
+    necR r_mapsto r_mapsto' ->
+    address_mapsto m v sh lbase r_mapsto' <->
+    address_mapsto m v sh lbase r_mapsto.
+Proof.
+  intros. apply necR_power_age in H.
+  destruct H as [n H]. revert dependent r_mapsto'.
+  revert dependent r_mapsto.
+  induction n;intros.
+  - inv H. subst. tauto.
+  - destruct H as [r_mapsto'' [? ?]].
+    apply IHn in H0. rewrite H0. clear H0.
+    hnf in H. split;intro.
+    { inv H0. exists x. destruct H1 as [[? ?] ?].
+      split;[split|].
+      + simpl. simpl in H0. auto.
+      + intros l. specialize (H1 l).
+        hnf in H1. hnf. if_tac.
+        { destruct H1. exists x0. hnf in H1.
+          hnf. simpl. epose proof age1_YES _ _ _ _ _ _ H.
+          apply H4 in H1. auto. }
+        { epose proof age1_resource_at_identity _ _ _ H.
+          apply H4 in H1. auto. }
+      + epose proof age1_ghost_of_identity _ _ H.
+        apply H3 in H2. auto.
+    }
+    { inv H0. exists x. destruct H1 as [[? ?] ?].
+      split;[split|].
+      + simpl. simpl in H0. auto.
+      + intros l. specialize (H1 l).
+        hnf in H1. hnf. if_tac.
+        { destruct H1. exists x0. hnf in H1.
+          hnf. simpl. epose proof age1_YES _ _ _ _ _ _ H.
+          apply H4 in H1. auto. }
+        { epose proof age1_resource_at_identity _ _ _ H.
+          apply H4 in H1. auto. }
+      + epose proof age1_ghost_of_identity _ _ H.
+        apply H3 in H2. auto.
+    }
+Qed.
+
+
+Lemma identity_resource_at_approx:
+  forall phi l,
+      resource_fmap (approx (level phi)) (approx (level phi)) (identity_resource_of (phi @ l)) = (identity_resource_of (phi @ l)).
+Proof.
+  intros. symmetry. rewrite rmap_level_eq. unfold resource_at.
+  case_eq (unsquash phi); intros.
+  simpl.
+  set (phi' := (squash (n, (resource_fmap (approx n) (approx n) oo fst r, snd r)))).
+  pose proof I.
+  generalize (unsquash_inj phi phi'); intro.
+  spec H1.
+  replace (unsquash phi) with (unsquash (squash (unsquash phi))).
+  2: rewrite squash_unsquash; auto.
+  rewrite H.
+  unfold phi'.
+  repeat rewrite unsquash_squash.
+  simpl.
+  f_equal.
+  unfold rmap_fmap, compose; simpl.
+  f_equal.
+  extensionality y.
+  rewrite resource_fmap_fmap.
+  rewrite approx_oo_approx; auto.
+  unfold phi' in *; clear phi'.
+  subst.
+  rewrite unsquash_squash in H.
+  injection H; clear H; intro.
+  pattern r at 1; rewrite <- H.
+  unfold rmap_fmap, compose.
+  simpl; rewrite resource_fmap_fmap.
+  rewrite approx_oo_approx; auto.
+  destruct (fst r l);simpl;reflexivity.
+Qed.
+
+Lemma two_share_join: forall sh1 sh2,
+join sh1 (Share.glb (Share.comp sh1) sh2) (Share.lub sh1 sh2).
+Proof.
+  intros. split.
+  - rewrite <- Share.glb_assoc. rewrite Share.comp2.
+    rewrite Share.glb_commute. rewrite Share.glb_bot. reflexivity.
+  - rewrite Share.distrib2. rewrite Share.comp1.
+    rewrite Share.glb_commute. rewrite Share.glb_top. reflexivity.
+Qed.
+
+
+Lemma cut_resource_rejoin_merge: 
+forall sh1 sh2 lbase m r (Q1 Q2: pred rmap)
+  (wsh1: writable_share sh1) (wsh2: writable_share sh2)
+  (Hw1: forall v' r', cut_resource_rejoin sh1 lbase m v' r r' -> Q1 r')
+  (Hw2: forall v' r', cut_resource_rejoin sh2 lbase m v' r r' -> Q2 r'),
+    (forall v' r', cut_resource_rejoin (Share.lub sh1 sh2) lbase m v' r r' -> Q1 r').
+Proof.
+  intros.
+  inv H. pose proof sepalg_list.nec_join3 H3 H2.
+  destruct H as [r_mapsto'' [r'' [? [? ?]]]].
+  eapply pred_nec_hereditary; try eassumption.
+  eapply Hw1.
+  apply (@address_mapsto_preserve_necR 
+    (Share.lub sh1 sh2) lbase m v' _ _ H4) in H0.
+  clear dependent r_rem'.
+  clear dependent r_mapsto'. clear  dependent r'.
+  assert (rsh1: readable_share sh1). 
+  { apply writable_readable_share. auto. }
+  assert (nsh2: ~ readable_share (Share.glb (Share.comp sh1) sh2)).
+  { intros C. eapply join_writable_readable.
+    2:{ apply wsh1. } 2:{ apply C. }
+    apply two_share_join. }
+  inversion H0 as [bm].
+  inv H1. inv H3.
+  remember (squash (level r_rem,(fun l =>
+    if (adr_range_dec lbase (size_chunk m) l) 
+    then YES sh1 rsh1 (VAL (nth (Z.to_nat (snd l - snd lbase)) bm Undef)) NoneP
+    else (r_mapsto'' @ l)
+  ,ghost_of r_mapsto''))) as r_maps1''.
+  remember (squash (level r_rem,(fun l =>
+    if (adr_range_dec lbase (size_chunk m) l) 
+    then YES sh1 rsh1 (VAL (nth (Z.to_nat (snd l - snd lbase)) bl Undef)) NoneP
+    else (r_mapsto @ l)
+  ,ghost_of r_mapsto))) as r_maps1.
+  remember (squash (level r_rem,(fun l =>
+    if (adr_range_dec lbase (size_chunk m) l) 
+    then NO (Share.glb (Share.comp sh1) sh2) nsh2 
+    else identity_resource_of (r_mapsto @ l)
+  ,nil))) as r_rem2.
+
+  assert (E1: join r_rem2 r_maps1'' r_mapsto'').
+  { apply join_unsquash. subst.
+    rewrite !unsquash_squash. split.
+    - simpl. apply join_level in H.
+       rewrite rmap_level_eq in *.
+       constructor;omega.
+    - split.
+      + simpl. unfold join. unfold Join_pi. 
+        intros l. unfold compose. simpl.
+        destruct H2 as [[? ?] ?].
+        specialize (H3 l). simpl in H3. if_tac.
+        { simpl. destruct H3. unfold resource_at in H3.
+          rewrite H3. constructor.
+          apply join_comm. apply two_share_join. }
+        { destruct H1. specialize (H1 l). simpl in H1.
+          assert (level r_rem = level r_mapsto).
+          { apply join_level in H4. omega. }
+          rewrite H8. rewrite identity_resource_at_approx. clear H8.
+          assert (level r_mapsto = level r_mapsto'').
+          { apply join_level in H. apply join_level in H4. omega. }
+          rewrite H8. rewrite resource_at_approx. clear H8.
+          unfold resource_at.
+          pose proof resource_at_join _ _ _ l H as Et1.
+          pose proof resource_at_join _ _ _ l H4 as Et2.
+          if_tac in H1; try tauto.
+          pose proof H1 _ _ Et2. apply join_comm in Et1.
+          pose proof H3 _ _ Et1. rewrite H9 in *. rewrite H10 in *.
+          unfold resource_at in Et1, Et2. clear H9. clear H10.
+          destruct ((fst (snd (unsquash r_mapsto)) l));simpl;
+          destruct ((fst (snd (unsquash r_mapsto'')) l));simpl;try constructor;try apply bot_join_eq; try solve [inv Et1; inv Et2; congruence].
+          inv Et1. inv Et2. rewrite H12. rewrite <- H13. constructor.
+        }
+      + simpl. assert (level r_rem = level r_mapsto'').
+        { apply join_level in H. omega. }
+        rewrite H3. rewrite ghost_of_approx. unfold ghost_of.
+        constructor.
+  }
+
+  assert (E2: join r_rem2 r_maps1 r_mapsto).
+  { apply join_unsquash. subst.
+    rewrite !unsquash_squash. split.
+    - simpl. apply join_level in H4.
+       rewrite rmap_level_eq in *.
+       constructor;omega.
+    - split.
+      + simpl. unfold join. unfold Join_pi. 
+        intros l. unfold compose. simpl.
+        destruct H2 as [[? ?] ?].
+        destruct H1. specialize (H1 l). simpl in H1.
+        if_tac.
+        { simpl. destruct H1. unfold resource_at in H1.
+          rewrite H1. constructor. apply join_comm.
+          apply two_share_join. }
+        { assert (level r_rem = level r_mapsto).
+          { apply join_level in H4. omega. }
+          rewrite H8. rewrite identity_resource_at_approx. clear H8.
+          rewrite resource_at_approx. apply join_comm.
+          apply identity_resource_of_sem. }
+      + simpl. assert (level r_rem = level r_mapsto).
+        { apply join_level in H4. omega. }
+        rewrite H3. rewrite ghost_of_approx. unfold ghost_of.
+        constructor.
+  }
+  assert (E3: address_mapsto m v' sh1 lbase r_maps1'').
+  { rewrite Heqr_maps1''. destruct H2 as [[? ?] ?].
+    exists bm. split;[split|].
+    - simpl. simpl in H2. auto.
+    - intros l. simpl. if_tac.
+      { exists rsh1. unfold resource_at. rewrite unsquash_squash.
+        simpl. unfold compose. if_tac;try tauto. }
+      { unfold resource_at. rewrite unsquash_squash. simpl.
+        unfold compose. if_tac; try tauto.
+        assert (level r_rem = level r_mapsto'').
+        { apply join_level in H. omega. }
+        rewrite H8. replace (fst (snd (unsquash r_mapsto'')) l) with
+        (r_mapsto'' @ l) by reflexivity.
+        rewrite resource_at_approx.
+        specialize (H3 l). simpl in H3. if_tac in H3;try tauto. }
+    - simpl. unfold ghost_of. rewrite unsquash_squash.
+      simpl. 
+      assert (level r_rem = level r_mapsto'').
+      { apply join_level in H4. apply join_level in H. omega. }
+      rewrite H6. rewrite ghost_of_approx. auto.
+  }
+  
+
+  apply join_comm in H.  apply join_comm in E1. apply join_comm in E2.
+  destruct (join_assoc E1 H) as [r_rm [HJ1 HJ2]].
+  destruct (join_assoc E2 H4) as [r_rm'' [HJ3 HJ4]].
+  assert (r_rm = r_rm'').
+  { eapply join_eq;eassumption. }
+  subst r_rm''. clear HJ3.
+  econstructor.
+  4:{ apply join_comm in HJ2. apply HJ2. }
+  3:{ apply necR_refl. }
+  { apply E3. }
+  { exists bl.
+    apply cut_resource_exp_intro with 
+     (r_mapsto:=r_maps1);auto. subst r_maps1.
+    split.
+    - intros l. simpl. if_tac.
+      { exists rsh1. unfold resource_at. rewrite unsquash_squash.
+        simpl. unfold compose. if_tac;try tauto. }
+      { unfold resource_at. rewrite unsquash_squash. simpl.
+        unfold compose. if_tac; try tauto.
+        assert (level r_rem = level r_mapsto).
+        { apply join_level in H4. omega. }
+        rewrite H6. replace (fst (snd (unsquash r_mapsto)) l) with
+        (r_mapsto @ l) by reflexivity.
+        rewrite resource_at_approx. destruct H1.
+        specialize (H1 l). simpl in H1. if_tac in H1;try tauto. }
+    - simpl. unfold ghost_of. rewrite unsquash_squash.
+      simpl. 
+      assert (level r_rem = level r_mapsto).
+      { apply join_level in H4. omega. }
+      rewrite H3. rewrite ghost_of_approx. destruct H1. auto.
+  }
+Qed.
+
+
 Lemma cut_resource_join: forall sh1 sh2 lbase len r1 r2 r
 (rsh1: readable_share sh1) (rsh2: readable_share sh2),
 cut_resource_rmap sh1 lbase len r1 r ->
 cut_resource_rmap sh2 lbase len r2 r ->
-exists r3, cut_resource_rmap (Share.lub sh1 sh2) lbase len r3 r  /\
-join_sub r3 r1.
+exists r3, cut_resource_rmap (Share.lub sh1 sh2) lbase len r3 r.
 Proof.
   intros.
   inversion H as [b1 ? ? H']. subst.
@@ -731,8 +981,7 @@ Proof.
               | left i => join_rem_of sh1 sh2 (r @ l) (JS1 l i) (JS2 l i)
               | right _ => (r @ l) end),
     ghost_of r1))).
-  split.
-  * apply cut_resource_intro with (bl:=b1).
+  apply cut_resource_intro with (bl:=b1).
     apply cut_resource_exp_intro with
     (r_mapsto:= (squash (level r, (
       (fun l => if (adr_range_dec lbase (Z.of_nat (Datatypes.length b1)) l)
@@ -803,7 +1052,8 @@ Proof.
           2:{ apply join_level in HJ1. omega. }
           rewrite ghost_of_approx. apply ghost_of_join.
           auto. }
-  * assert (JS3: forall l, adr_range lbase (Z.of_nat (Datatypes.length b1)) l 
+Qed.
+  (* * assert (JS3: forall l, adr_range lbase (Z.of_nat (Datatypes.length b1)) l 
       -> join_sub (Share.glb (share_of (r1 @ l)) (Share.comp sh2)) (share_of (r1 @ l))).
     { intros. exists (Share.glb (share_of (r1 @ l)) sh2).
       split.
@@ -858,7 +1108,7 @@ Proof.
             destruct (r1@l) eqn:E';simpl.
             - destruct (dec_readable sh0);try contradiction.
               destruct dec_readable;simpl.
-              destruct Hml1. Admitted.
+              destruct Hml1. Admitted. *)
 (* 
       }
       { simpl.
@@ -902,9 +1152,6 @@ Proof.
    intros.
   
   ) *)
-
-
-
 
 
 Lemma list_nth_eq': forall {A:Type} (l1 l2: list A) d,
@@ -998,8 +1245,7 @@ join r2_maps r2_rem r ->
 address_mapsto m v1 sh1 (b, Ptrofs.unsigned i) r1_maps ->
 address_mapsto m v2 sh2 (b, Ptrofs.unsigned i) r2_maps ->
 v1 = v2 /\ exists r_maps r_rem, join r_maps r_rem r /\
-address_mapsto m v1 (Share.lub sh1 sh2) (b, Ptrofs.unsigned i) r_maps /\
-join_sub r_rem r1_rem /\ join_sub r_rem r2_rem.
+address_mapsto m v1 (Share.lub sh1 sh2) (b, Ptrofs.unsigned i) r_maps.
 Proof.
 intros.
 pose proof address_mapsto_join_value
@@ -1021,9 +1267,9 @@ assert (cut_resource_rmap_exp sh2 (b, Ptrofs.unsigned i) (size_chunk m) bm2 r2_r
 }
 apply cut_resource_intro in H3. apply cut_resource_intro in H4.
 pose proof cut_resource_join _ _ _ _ _ _ _ H H0 H3 H4.
-destruct H5 as [r_rem [H5 Ht]]. pose proof H5 as H5'.
+destruct H5 as [r_rem H5]. pose proof H5 as H5'.
 inv H5. inv H6.
-exists r_mapsto, r_rem. split;auto. split.
+exists r_mapsto, r_rem. split;auto.
 hnf. exists bl. destruct H5. repeat split;auto.
 + unfold size_chunk_nat.
   rewrite <- (Nat2Z.id (Datatypes.length bl)).
@@ -1040,13 +1286,6 @@ hnf. exists bl. destruct H5. repeat split;auto.
     pose proof address_mapsto_join_value
     _ _ _ _ _ _ _ _ _ _ _ H1 H7 H9 H8.
     auto.
-+ split;auto.
-  pose proof cut_resource_join _ _ _ _ _ _ _ H0 H H4 H3.
-  destruct H6 as [r_rem' [H6 Ht']].
-  rewrite Share.lub_commute in H6.
-  rewrite (cut_resource_rmap_unique _ _ _ _ _ _ H6 H5') in *.
-  (* use unique + symetric property to avoid redundant proof *)
-  auto.
 Qed.
 
 
@@ -1098,7 +1337,6 @@ Proof.
     split. 2:{ simpl. auto. }
     exists r_maps, r_rem. repeat split;auto. left.
     split;auto.
-    tauto.
   }
 Qed.
 
@@ -1130,40 +1368,102 @@ writable_share sh1 -> writable_share sh2 ->
 |-- EX (sh':share), 
 (mapsto_ sh' t p * (ALL v', mapsto sh' t p v' -* (P1 && P2))).
 Proof.
-intros sh1 sh2 t p P1 P2 Hsh1w Hsh2w. unfold mapsto_. unfold mapsto.
-pose proof writable_readable_share Hsh1w as Hsh1.
-pose proof writable_readable_share Hsh2w as Hsh2.
-destruct (access_mode t); try solve [rewrite FF_sepcon; rewrite FF_and; auto].
-destruct (type_is_volatile t); try solve [rewrite FF_sepcon; rewrite FF_and; auto].
-destruct p; try solve [rewrite FF_sepcon; rewrite FF_and; auto].
-if_tac; try tauto. if_tac; try tauto.
-hnf. intros r.
-intros [E1 E2].
-destruct E1 as [r1_maps [r1_rem [Ea1 [Eb1 Ec1]]]].
-destruct E2 as [r2_maps [r2_rem [Ea2 [Eb2 Ec2]]]].
-destruct Eb1 as [Eb1 | Eb1].
-{ destruct Eb1 as [H1 ?]. exfalso. eapply tc_val_Vundef. apply H1. }
-destruct Eb1 as [_ Eb1]. destruct Eb1 as [v1 Eb1].
-destruct Eb2 as [Eb2 | Eb2].
-{ destruct Eb2 as [H1 ?]. exfalso. eapply tc_val_Vundef. apply H1. }
-destruct Eb2 as [_ Eb2]. destruct Eb2 as [v2 Eb2].
-{ pose proof address_mapsto_join
-      _ _ _ _ _ _ _ _ _ _ _ _ Hsh1 Hsh2 Ea1 Ea2 Eb1 Eb2.
-  destruct H1. subst v2.
-  destruct H2 as [r_maps [r_rem [E1 E2]]].
-  exists (Share.lub sh1 sh2).
-  if_tac.
-  2:{ exfalso. apply H1. apply readable_share_lub. auto. }
-  exists r_maps, r_rem. split;auto.
-  split.
-  - right. split. { simpl. auto. } exists v1. tauto.
-  - intros v'. destruct E2 as [E2 [E3 E4]]. intros r_rem' r_maps' r'.
-    intros. split.
-    + assert (H5: exists v', address_mapsto m v' (Share.lub sh1 sh2) (b, Ptrofs.unsigned i) r_maps').
+  intros sh1 sh2 t p P1 P2 Hsh1w Hsh2w. unfold mapsto_. unfold mapsto.
+  pose proof writable_readable_share Hsh1w as Hsh1.
+  pose proof writable_readable_share Hsh2w as Hsh2.
+  destruct (access_mode t); try solve [rewrite FF_sepcon; rewrite FF_and; auto].
+  destruct (type_is_volatile t); try solve [rewrite FF_sepcon; rewrite FF_and; auto].
+  destruct p; try solve [rewrite FF_sepcon; rewrite FF_and; auto].
+  if_tac; try tauto. if_tac; try tauto.
+  hnf. intros r.
+  intros [E1 E2].
+  destruct E1 as [r1_maps [r1_rem [Ea1 [Eb1 Ec1]]]].
+  destruct E2 as [r2_maps [r2_rem [Ea2 [Eb2 Ec2]]]].
+  destruct Eb1 as [Eb1 | Eb1].
+  { destruct Eb1 as [H1 ?]. exfalso. eapply tc_val_Vundef. apply H1. }
+  destruct Eb1 as [_ Eb1]. destruct Eb1 as [v1 Eb1].
+  destruct Eb2 as [Eb2 | Eb2].
+  { destruct Eb2 as [H1 ?]. exfalso. eapply tc_val_Vundef. apply H1. }
+  destruct Eb2 as [_ Eb2]. destruct Eb2 as [v2 Eb2].
+  { pose proof address_mapsto_join
+        _ _ _ _ _ _ _ _ _ _ _ _ Hsh1 Hsh2 Ea1 Ea2 Eb1 Eb2.
+    destruct H1. subst v2.
+    destruct H2 as [r_maps [r_rem [E1 E2]]].
+    assert (EP1: forall v' r', cut_resource_rejoin sh1 
+                    (b, Ptrofs.unsigned i) m v' r r' -> P1 r').
+    { intros v'. eapply cut_resource_sem.
+      exists r1_maps, r1_rem.
+      split;auto. split;try eassumption.
+      hnf. intros.
+      eapply Ec1. { apply H1. } { apply H2. }
+      { right. split. 2:{ exists v'. auto. } reflexivity. }
+    }
+    assert (EP2: forall v' r', cut_resource_rejoin sh2
+                    (b, Ptrofs.unsigned i) m v' r r' -> P2 r').
+    { intros v'. eapply cut_resource_sem.
+      exists r2_maps, r2_rem.
+      split;auto. split;try eassumption.
+      hnf. intros.
+      eapply Ec2. { apply H1. } { apply H2. }
+      { right. split. 2:{ exists v'. auto. } reflexivity. }
+    }
+    exists (Share.lub sh1 sh2).
+    if_tac.
+    2:{ exfalso. apply H1. apply readable_share_lub. auto. }
+    exists r_maps, r_rem. split;auto.
+    split.
+    - right. split. { simpl. auto. } exists v1. tauto.
+    - intros v'.
+      pose proof cut_resource_rejoin_merge
+         _ _ _ _ _ _ _ Hsh1w Hsh2w EP1 EP2 as T1.
+      pose proof cut_resource_rejoin_merge
+         _ _ _ _ _ _ _ Hsh2w Hsh1w EP2 EP1 as T2.
+      rewrite Share.lub_commute in T2.
+      hnf. intros. split.
       { destruct H4.
-        - destruct H4. exists v'. auto.
-        - destruct H4. destruct H5. exists x. auto. }
-      clear H4 v'.  destruct H5 as [v' H4].
+        + destruct H4. eapply T1 with (v':=v').
+          econstructor; try eassumption.
+          destruct E2 as [bl [[?E ?E] ?E]]. exists bl.
+          econstructor. 3:{ apply E1. }
+          2:{ split;auto. }
+          destruct E. rewrite size_chunk_conv.
+          rewrite H6. reflexivity.
+        + destruct H4. clear H4. destruct H5.
+          eapply T1 with (v':=x).
+          econstructor; try eassumption.
+          destruct E2 as [bl [[?E ?E] ?E]]. exists bl.
+          econstructor. 3:{ apply E1. }
+          2:{ split;auto. }
+          destruct E. rewrite size_chunk_conv.
+          rewrite H5. reflexivity.
+      }
+      { destruct H4.
+        + destruct H4. eapply T2 with (v':=v').
+          econstructor; try eassumption.
+          destruct E2 as [bl [[?E ?E] ?E]]. exists bl.
+          econstructor. 3:{ apply E1. }
+          2:{ split;auto. }
+          destruct E. rewrite size_chunk_conv.
+          rewrite H6. reflexivity.
+        + destruct H4. clear H4. destruct H5.
+          eapply T2 with (v':=x).
+          econstructor; try eassumption.
+          destruct E2 as [bl [[?E ?E] ?E]]. exists bl.
+          econstructor. 3:{ apply E1. }
+          2:{ split;auto. }
+          destruct E. rewrite size_chunk_conv.
+          rewrite H5. reflexivity.
+      }
+  }
+Qed.
+    
+    (* destruct E2 as [E2 [E3 E4]]. intros r_rem' r_maps' r'.
+      intros. split.
+      + assert (H5: exists v', address_mapsto m v' (Share.lub sh1 sh2) (b, Ptrofs.unsigned i) r_maps').
+        { destruct H4.
+          - destruct H4. exists v'. auto.
+          - destruct H4. destruct H5. exists x. auto. }
+        clear H4 v'.  destruct H5 as [v' H4].
       assert (exists r_maps1' r_maps2',
         join r_maps1' r_maps2' r_maps' /\
         address_mapsto m v' sh1 (b, Ptrofs.unsigned i) r_maps1'
@@ -1215,9 +1515,7 @@ destruct Eb2 as [_ Eb2]. destruct Eb2 as [v2 Eb2].
 
 
 
-  split;auto.
-}
-Qed.
+  split;auto. *)
 
 Lemma necR_split_1n: forall n r1 r2,
 relation_power (S n) age r1 r2 -> exists y, age r1 y /\ necR y r2.
